[axe/x86] Implement new scheme for 32-bit registers.
Now, for 32-bit proofs, the register getters and setters in our normal form deal only with the low 32-bits of each register.  Because the 32-bit instructions can affect bits above these (due to code reuse from the 64-bit instructions), we introduce machinery to reason about the high half of the registers.  The 32-bit instructions seem to either preserve these bits or set them to 0, so we add assumptions that these bits are initially 0 (in 32-bit mode, where they are irrelevant).  These new assumptions allow rewrite rules to simplify away the functions affecting the high halves of the registers.

books/kestrel/x86/register-readers-and-writers32.lisp
@@ -21,47 +21,170 @@
 (include-book "projects/x86isa/machine/state" :dir :system) ;for xr
 (include-book "projects/x86isa/portcullis/sharp-dot-constants" :dir :system)
 (include-book "kestrel/bv/bvchop-def" :dir :system)
+(include-book "kestrel/bv/bvcat-def" :dir :system)
+(include-book "kestrel/bv/slice-def" :dir :system)
+(local (include-book "kestrel/bv/rules" :dir :system)) ; for bvcat-of-logext-arg4
 (local (include-book "kestrel/bv/logext" :dir :system))
+(local (include-book "kestrel/bv/bvchop" :dir :system))
+(local (include-book "kestrel/bv/bvcat" :dir :system))
 
 (in-theory (disable xw logext))
 
-;; Register readers
-(defund eax (x86) (declare (xargs :stobjs x86)) (rgfi *rax* x86))
-(defund ebx (x86) (declare (xargs :stobjs x86)) (rgfi *rbx* x86))
-(defund ecx (x86) (declare (xargs :stobjs x86)) (rgfi *rcx* x86))
-(defund edx (x86) (declare (xargs :stobjs x86)) (rgfi *rdx* x86))
-(defund esp (x86) (declare (xargs :stobjs x86)) (rgfi *rsp* x86))
-(defund ebp (x86) (declare (xargs :stobjs x86)) (rgfi *rbp* x86))
+(defthm xw-of-rgf-and-logext64
+  (equal (xw :rgf reg (logext 64 val) x86)
+         (xw :rgf reg val x86))
+  :hints (("Goal" :in-theory (enable xw))))
+
+;;;;;;;;;;;;;;;;;;;;;;;;;;;;;;;;;;;;;;;;;;;;;;;;;;;;;;;;;;;;;;;;;;;;;;;;;;;;;;;;
+
+;; Helpers for expressing the high bits of the 64-bit registers (in 32-bit mode, these are usually ignored).
+;; todo: just make a single one of these?
+(defund rax-high (x86) (declare (xargs :stobjs x86)) (slice 63 32 (rgfi *rax* x86)))
+(defund rbx-high (x86) (declare (xargs :stobjs x86)) (slice 63 32 (rgfi *rbx* x86)))
+(defund rcx-high (x86) (declare (xargs :stobjs x86)) (slice 63 32 (rgfi *rcx* x86)))
+(defund rdx-high (x86) (declare (xargs :stobjs x86)) (slice 63 32 (rgfi *rdx* x86)))
+(defund rsp-high (x86) (declare (xargs :stobjs x86)) (slice 63 32 (rgfi *rsp* x86)))
+(defund rbp-high (x86) (declare (xargs :stobjs x86)) (slice 63 32 (rgfi *rbp* x86)))
+
+;; Register readers (these take the signed-byte-64 values and chop them down to unsigned-byte-32s):
+(defund eax (x86) (declare (xargs :stobjs x86)) (bvchop 32 (rgfi *rax* x86)))
+(defund ebx (x86) (declare (xargs :stobjs x86)) (bvchop 32 (rgfi *rbx* x86)))
+(defund ecx (x86) (declare (xargs :stobjs x86)) (bvchop 32 (rgfi *rcx* x86)))
+(defund edx (x86) (declare (xargs :stobjs x86)) (bvchop 32 (rgfi *rdx* x86)))
+(defund esp (x86) (declare (xargs :stobjs x86)) (bvchop 32 (rgfi *rsp* x86)))
+(defund ebp (x86) (declare (xargs :stobjs x86)) (bvchop 32 (rgfi *rbp* x86)))
 ;; todo: esi and edi!
 
+;; Introduce the register readers:
+;; These rules are disabled since they are not appropriate for 64-bit reasoning:
+(defthmd xr-becomes-eax (equal (xr :rgf *rax* x86) (logext 64 (bvcat 32 (rax-high x86) 32 (eax x86)))) :hints (("Goal" :in-theory (enable eax rax-high))))
+(defthmd xr-becomes-ebx (equal (xr :rgf *rbx* x86) (logext 64 (bvcat 32 (rbx-high x86) 32 (ebx x86)))) :hints (("Goal" :in-theory (enable ebx rbx-high))))
+(defthmd xr-becomes-ecx (equal (xr :rgf *rcx* x86) (logext 64 (bvcat 32 (rcx-high x86) 32 (ecx x86)))) :hints (("Goal" :in-theory (enable ecx rcx-high))))
+(defthmd xr-becomes-edx (equal (xr :rgf *rdx* x86) (logext 64 (bvcat 32 (rdx-high x86) 32 (edx x86)))) :hints (("Goal" :in-theory (enable edx rdx-high))))
+(defthmd xr-becomes-esp (equal (xr :rgf *rsp* x86) (logext 64 (bvcat 32 (rsp-high x86) 32 (esp x86)))) :hints (("Goal" :in-theory (enable esp rsp-high))))
+(defthmd xr-becomes-ebp (equal (xr :rgf *rbp* x86) (logext 64 (bvcat 32 (rbp-high x86) 32 (ebp x86)))) :hints (("Goal" :in-theory (enable ebp rbp-high))))
+
+(theory-invariant (incompatible (:definition eax) (:rewrite xr-becomes-eax)))
+(theory-invariant (incompatible (:definition ebx) (:rewrite xr-becomes-ebx)))
+(theory-invariant (incompatible (:definition ecx) (:rewrite xr-becomes-ecx)))
+(theory-invariant (incompatible (:definition edx) (:rewrite xr-becomes-edx)))
+(theory-invariant (incompatible (:definition esp) (:rewrite xr-becomes-esp)))
+(theory-invariant (incompatible (:definition ebp) (:rewrite xr-becomes-ebp)))
+
+;;;;;;;;;;;;;;;;;;;;;;;;;;;;;;;;;;;;;;;;;;;;;;;;;;;;;;;;;;;;;;;;;;;;;;;;;;;;;;;;
+
+;; Aliases for expressing the high bits of the 48-bit RIP (undefined in 32-bit mode).
+(defund rip-high (x86) (declare (xargs :stobjs x86)) (slice 47 32 (rip x86)))
+
 ;; Gets the 32-bit instruction pointer:
-(defun eip (x86)
-  (declare (xargs :stobjs x86))
-  (rip x86))
+(defun eip (x86) (declare (xargs :stobjs x86)) (bvchop 32 (rip x86)))
 
-(defthmd xr-becomes-eip
-  (equal (xr :rip nil x86) (eip x86))
-  :hints (("Goal" :in-theory (enable eip rip))))
+;; These rules are disabled since they are not appropriate for 64-bit reasoning:
+(defthmd rip-becomes-eip (equal (rip x86) (logext 48 (bvcat 16 (rip-high x86) 32 (eip x86)))) :hints (("Goal" :in-theory (enable eip rip-high))))
+(defthmd xr-becomes-eip (equal (xr :rip nil x86) (logext 48 (bvcat 16 (rip-high x86) 32 (eip x86)))) :hints (("Goal" :in-theory (enable eip rip-high))))
 
-(defthmd rip-becomes-eip
-  (equal (rip x86) (eip x86))
-  :hints (("Goal" :in-theory (enable eip))))
+(theory-invariant (incompatible (:rewrite rip-becomes-eip) (:definition eip)))
+(theory-invariant (incompatible (:rewrite xr-becomes-eip) (:definition eip)))
 
 ;; not quite true
 ;; (defthm read-*ip-of-*compatibility-mode*-becomes-eip
 ;;   (equal (read-*ip *compatibility-mode* x86) (eip x86))
 ;;   :hints (("Goal" :in-theory (enable read-*ip))))
 
-(theory-invariant (incompatible (:rewrite rip-becomes-eip) (:definition eip)))
-(theory-invariant (incompatible (:rewrite xr-becomes-eip) (:definition eip)))
+;;;;;;;;;;;;;;;;;;;;;;;;;;;;;;;;;;;;;;;;;;;;;;;;;;;;;;;;;;;;;;;;;;;;;;;;;;;;;;;;
 
-;; Register writers
-(defund set-eax (val x86) (declare (xargs :stobjs x86 :guard (unsigned-byte-p 32 val))) (!rgfi *rax* val x86))
-(defund set-ebx (val x86) (declare (xargs :stobjs x86 :guard (unsigned-byte-p 32 val))) (!rgfi *rbx* val x86))
-(defund set-ecx (val x86) (declare (xargs :stobjs x86 :guard (unsigned-byte-p 32 val))) (!rgfi *rcx* val x86))
-(defund set-edx (val x86) (declare (xargs :stobjs x86 :guard (unsigned-byte-p 32 val))) (!rgfi *rdx* val x86))
-(defund set-esp (val x86) (declare (xargs :stobjs x86 :guard (unsigned-byte-p 32 val))) (!rgfi *rsp* val x86))
-(defund set-ebp (val x86) (declare (xargs :stobjs x86 :guard (unsigned-byte-p 32 val))) (!rgfi *rbp* val x86))
+;; Helpers for the high bits (usually unused in 32-bit mode):
+(defund set-reg-high (reg val x86)
+  (declare (xargs :stobjs x86 :guard (and (and (natp reg) (< reg 16))
+                                          (unsigned-byte-p 32 val))))
+  (!rgfi reg (logext 64 (bvcat 32 val 32 (rgfi reg x86))) x86))
+
+(defthm set-reg-high-of-set-reg-high-same
+  (equal (set-reg-high reg val1 (set-reg-high reg val2 x86))
+         (set-reg-high reg val1 x86))
+  :hints (("Goal" :in-theory (enable set-reg-high
+                                     acl2::bvcat-of-bvcat-tighten-arg4))))
+
+(defthm set-reg-high-of-set-reg-high-diff
+  (implies (< reg2 reg1)
+           (equal (set-reg-high reg1 val1 (set-reg-high reg2 val2 x86))
+                  (set-reg-high reg2 val2 (set-reg-high reg1 val1 x86))))
+  :hints (("Goal" :in-theory (enable set-reg-high))))
+
+(defthm set-reg-high-of-bvchop (implies (and (<= 32 n) (integerp n)) (equal (set-reg-high reg (bvchop n val) x86) (set-reg-high reg val x86))) :hints (("Goal" :in-theory (enable set-reg-high))))
+(defthm set-reg-high-does-nothing (implies (equal val (slice 63 32 (rgfi reg x86))) (equal (set-reg-high reg val x86) x86)) :hints (("Goal" :in-theory (enable set-reg-high))))
+
+;; todo: either make separate set-reg-high functions for each register, or don't have separate getters like rax-high
+(defthm set-reg-high-of-rax-does-nothing (implies (equal val (rax-high x86)) (equal (set-reg-high *rax* val x86) x86)) :hints (("Goal" :in-theory (enable rax-high set-reg-high))))
+(defthm set-reg-high-of-rbx-does-nothing (implies (equal val (rbx-high x86)) (equal (set-reg-high *rbx* val x86) x86)) :hints (("Goal" :in-theory (enable rbx-high set-reg-high))))
+(defthm set-reg-high-of-rcx-does-nothing (implies (equal val (rcx-high x86)) (equal (set-reg-high *rcx* val x86) x86)) :hints (("Goal" :in-theory (enable rcx-high set-reg-high))))
+(defthm set-reg-high-of-rdx-does-nothing (implies (equal val (rdx-high x86)) (equal (set-reg-high *rdx* val x86) x86)) :hints (("Goal" :in-theory (enable rdx-high set-reg-high))))
+(defthm set-reg-high-of-rsp-does-nothing (implies (equal val (rsp-high x86)) (equal (set-reg-high *rsp* val x86) x86)) :hints (("Goal" :in-theory (enable rsp-high set-reg-high))))
+(defthm set-reg-high-of-rbp-does-nothing (implies (equal val (rbp-high x86)) (equal (set-reg-high *rbp* val x86) x86)) :hints (("Goal" :in-theory (enable rbp-high set-reg-high))))
+
+(defthm x86p-of-set-reg-high (implies (x86p x86) (x86p (set-reg-high reg val x86))) :hints (("Goal" :in-theory (enable set-reg-high))))
+(defthm eip-of-set-reg-high (equal (eip (set-reg-high reg val x86)) (eip x86)) :hints (("Goal" :in-theory (enable set-reg-high))))
+;; todo: more like this?
+
+;; (defund set-rax-high (val x86) (declare (xargs :stobjs x86 :guard (unsigned-byte-p 32 val))) (!rgfi *rax* (logext 64 (bvcat 32 val 32 (rgfi *rax* x86))) x86))
+;; (defund set-rbx-high (val x86) (declare (xargs :stobjs x86 :guard (unsigned-byte-p 32 val))) (!rgfi *rbx* (logext 64 (bvcat 32 val 32 (rgfi *rbx* x86))) x86))
+;; (defund set-rcx-high (val x86) (declare (xargs :stobjs x86 :guard (unsigned-byte-p 32 val))) (!rgfi *rcx* (logext 64 (bvcat 32 val 32 (rgfi *rcx* x86))) x86))
+;; (defund set-rdx-high (val x86) (declare (xargs :stobjs x86 :guard (unsigned-byte-p 32 val))) (!rgfi *rdx* (logext 64 (bvcat 32 val 32 (rgfi *rdx* x86))) x86))
+;; (defund set-rsp-high (val x86) (declare (xargs :stobjs x86 :guard (unsigned-byte-p 32 val))) (!rgfi *rsp* (logext 64 (bvcat 32 val 32 (rgfi *rsp* x86))) x86))
+;; (defund set-rbp-high (val x86) (declare (xargs :stobjs x86 :guard (unsigned-byte-p 32 val))) (!rgfi *rbp* (logext 64 (bvcat 32 val 32 (rgfi *rbp* x86))) x86))
+
+;; (defthm set-rax-high-of-bvchop (implies (and (<= 32 n) (integerp n)) (equal (set-rax-high (bvchop n val) x86) (set-rax-high val x86))) :hints (("Goal" :in-theory (enable set-rax-high))))
+;; (defthm set-rbx-high-of-bvchop (implies (and (<= 32 n) (integerp n)) (equal (set-rbx-high (bvchop n val) x86) (set-rbx-high val x86))) :hints (("Goal" :in-theory (enable set-rbx-high))))
+;; (defthm set-rcx-high-of-bvchop (implies (and (<= 32 n) (integerp n)) (equal (set-rcx-high (bvchop n val) x86) (set-rcx-high val x86))) :hints (("Goal" :in-theory (enable set-rcx-high))))
+;; (defthm set-rdx-high-of-bvchop (implies (and (<= 32 n) (integerp n)) (equal (set-rdx-high (bvchop n val) x86) (set-rdx-high val x86))) :hints (("Goal" :in-theory (enable set-rdx-high))))
+;; (defthm set-rsp-high-of-bvchop (implies (and (<= 32 n) (integerp n)) (equal (set-rsp-high (bvchop n val) x86) (set-rsp-high val x86))) :hints (("Goal" :in-theory (enable set-rsp-high))))
+;; (defthm set-rbp-high-of-bvchop (implies (and (<= 32 n) (integerp n)) (equal (set-rbp-high (bvchop n val) x86) (set-rbp-high val x86))) :hints (("Goal" :in-theory (enable set-rbp-high))))
+
+;; (defthm set-rax-high-does-nothing (implies (equal val (rax-high x86)) (equal (set-rax-high val x86) x86)) :hints (("Goal" :in-theory (enable rax-high set-rax-high))))
+;; (defthm set-rbx-high-does-nothing (implies (equal val (rbx-high x86)) (equal (set-rbx-high val x86) x86)) :hints (("Goal" :in-theory (enable rbx-high set-rbx-high))))
+;; (defthm set-rcx-high-does-nothing (implies (equal val (rcx-high x86)) (equal (set-rcx-high val x86) x86)) :hints (("Goal" :in-theory (enable rcx-high set-rcx-high))))
+;; (defthm set-rdx-high-does-nothing (implies (equal val (rdx-high x86)) (equal (set-rdx-high val x86) x86)) :hints (("Goal" :in-theory (enable rdx-high set-rdx-high))))
+;; (defthm set-rsp-high-does-nothing (implies (equal val (rsp-high x86)) (equal (set-rsp-high val x86) x86)) :hints (("Goal" :in-theory (enable rsp-high set-rsp-high))))
+;; (defthm set-rbp-high-does-nothing (implies (equal val (rbp-high x86)) (equal (set-rbp-high val x86) x86)) :hints (("Goal" :in-theory (enable rbp-high set-rbp-high))))
+
+;; Register writers (these only change the low 32 bits):
+(defund set-eax (val x86) (declare (xargs :stobjs x86 :guard (unsigned-byte-p 32 val))) (!rgfi *rax* (logext 64 (bvcat 32 (rax-high x86) 32 (bvchop 32 val))) x86)) ; could drop the bvchop
+(defund set-ebx (val x86) (declare (xargs :stobjs x86 :guard (unsigned-byte-p 32 val))) (!rgfi *rbx* (logext 64 (bvcat 32 (rbx-high x86) 32 (bvchop 32 val))) x86)) ; could drop the bvchop
+(defund set-ecx (val x86) (declare (xargs :stobjs x86 :guard (unsigned-byte-p 32 val))) (!rgfi *rcx* (logext 64 (bvcat 32 (rcx-high x86) 32 (bvchop 32 val))) x86)) ; could drop the bvchop
+(defund set-edx (val x86) (declare (xargs :stobjs x86 :guard (unsigned-byte-p 32 val))) (!rgfi *rdx* (logext 64 (bvcat 32 (rdx-high x86) 32 (bvchop 32 val))) x86)) ; could drop the bvchop
+(defund set-esp (val x86) (declare (xargs :stobjs x86 :guard (unsigned-byte-p 32 val))) (!rgfi *rsp* (logext 64 (bvcat 32 (rsp-high x86) 32 (bvchop 32 val))) x86)) ; could drop the bvchop
+(defund set-ebp (val x86) (declare (xargs :stobjs x86 :guard (unsigned-byte-p 32 val))) (!rgfi *rbp* (logext 64 (bvcat 32 (rbp-high x86) 32 (bvchop 32 val))) x86)) ; could drop the bvchop
+
+;; Introduce the register writers
+;; The extra calls of set-rax-high, etc. should usually be irrelevant (todo: add rules about that, also reading-the-read rules about those...)
+;; These rules are disabled since they are not appropriate for 64-bit reasoning:
+(defthmd xw-becomes-set-eax (equal (xw :rgf *rax* val x86) (set-eax (bvchop 32 val) (set-reg-high *rax* (slice 63 32 val) x86))) :hints (("Goal" :in-theory (enable set-eax rax-high set-reg-high))))
+(defthmd xw-becomes-set-ebx (equal (xw :rgf *rbx* val x86) (set-ebx (bvchop 32 val) (set-reg-high *rbx* (slice 63 32 val) x86))) :hints (("Goal" :in-theory (enable set-ebx rbx-high set-reg-high))))
+(defthmd xw-becomes-set-ecx (equal (xw :rgf *rcx* val x86) (set-ecx (bvchop 32 val) (set-reg-high *rcx* (slice 63 32 val) x86))) :hints (("Goal" :in-theory (enable set-ecx rcx-high set-reg-high))))
+(defthmd xw-becomes-set-edx (equal (xw :rgf *rdx* val x86) (set-edx (bvchop 32 val) (set-reg-high *rdx* (slice 63 32 val) x86))) :hints (("Goal" :in-theory (enable set-edx rdx-high set-reg-high))))
+(defthmd xw-becomes-set-esp (equal (xw :rgf *rsp* val x86) (set-esp (bvchop 32 val) (set-reg-high *rsp* (slice 63 32 val) x86))) :hints (("Goal" :in-theory (enable set-esp rsp-high set-reg-high))))
+(defthmd xw-becomes-set-ebp (equal (xw :rgf *rbp* val x86) (set-ebp (bvchop 32 val) (set-reg-high *rbp* (slice 63 32 val) x86))) :hints (("Goal" :in-theory (enable set-ebp rbp-high set-reg-high))))
+
+(theory-invariant (incompatible (:definition set-eax) (:rewrite xw-becomes-set-eax)))
+(theory-invariant (incompatible (:definition set-ebx) (:rewrite xw-becomes-set-ebx)))
+(theory-invariant (incompatible (:definition set-ecx) (:rewrite xw-becomes-set-ecx)))
+(theory-invariant (incompatible (:definition set-edx) (:rewrite xw-becomes-set-edx)))
+(theory-invariant (incompatible (:definition set-esp) (:rewrite xw-becomes-set-esp)))
+(theory-invariant (incompatible (:definition set-ebp) (:rewrite xw-becomes-set-ebp)))
+
+(defthm set-eax-of-bvchop (implies (and (<= 32 n) (integerp n)) (equal (set-eax (bvchop n val) x86) (set-eax val x86))) :hints (("Goal" :in-theory (enable set-eax))))
+(defthm set-ebx-of-bvchop (implies (and (<= 32 n) (integerp n)) (equal (set-ebx (bvchop n val) x86) (set-ebx val x86))) :hints (("Goal" :in-theory (enable set-ebx))))
+(defthm set-ecx-of-bvchop (implies (and (<= 32 n) (integerp n)) (equal (set-ecx (bvchop n val) x86) (set-ecx val x86))) :hints (("Goal" :in-theory (enable set-ecx))))
+(defthm set-edx-of-bvchop (implies (and (<= 32 n) (integerp n)) (equal (set-edx (bvchop n val) x86) (set-edx val x86))) :hints (("Goal" :in-theory (enable set-edx))))
+(defthm set-esp-of-bvchop (implies (and (<= 32 n) (integerp n)) (equal (set-esp (bvchop n val) x86) (set-esp val x86))) :hints (("Goal" :in-theory (enable set-esp))))
+(defthm set-ebp-of-bvchop (implies (and (<= 32 n) (integerp n)) (equal (set-ebp (bvchop n val) x86) (set-ebp val x86))) :hints (("Goal" :in-theory (enable set-ebp))))
+
+(defthm set-eax-when-equal-eax (implies (equal val (eax x86)) (equal (set-eax val x86) x86)) :hints (("Goal" :in-theory (enable rax-high eax set-eax))))
+(defthm set-ebx-when-equal-ebx (implies (equal val (ebx x86)) (equal (set-ebx val x86) x86)) :hints (("Goal" :in-theory (enable rbx-high ebx set-ebx))))
+(defthm set-ecx-when-equal-ecx (implies (equal val (ecx x86)) (equal (set-ecx val x86) x86)) :hints (("Goal" :in-theory (enable rcx-high ecx set-ecx))))
+(defthm set-edx-when-equal-edx (implies (equal val (edx x86)) (equal (set-edx val x86) x86)) :hints (("Goal" :in-theory (enable rdx-high edx set-edx))))
+(defthm set-esp-when-equal-esp (implies (equal val (esp x86)) (equal (set-esp val x86) x86)) :hints (("Goal" :in-theory (enable rsp-high esp set-esp))))
+(defthm set-ebp-when-equal-ebp (implies (equal val (ebp x86)) (equal (set-ebp val x86) x86)) :hints (("Goal" :in-theory (enable rbp-high ebp set-ebp))))
 
 (defun set-eip (eip x86)
   (declare (xargs :stobjs x86
@@ -82,15 +205,15 @@
 
 (defthm eip-of-set-eip
   (equal (eip (set-eip eip x86))
-         (logext 48 eip)))
+         (bvchop 32 eip)))
 
 ;; Read of a write of the same register
-(defthm eax-of-set-eax (equal (eax (set-eax val x86)) (logext 64 val)) :hints (("Goal" :in-theory (enable eax set-eax))))
-(defthm ebx-of-set-ebx (equal (ebx (set-ebx val x86)) (logext 64 val)) :hints (("Goal" :in-theory (enable ebx set-ebx))))
-(defthm ecx-of-set-ecx (equal (ecx (set-ecx val x86)) (logext 64 val)) :hints (("Goal" :in-theory (enable ecx set-ecx))))
-(defthm edx-of-set-edx (equal (edx (set-edx val x86)) (logext 64 val)) :hints (("Goal" :in-theory (enable edx set-edx))))
-(defthm esp-of-set-esp (equal (esp (set-esp val x86)) (logext 64 val)) :hints (("Goal" :in-theory (enable esp set-esp))))
-(defthm ebp-of-set-ebp (equal (ebp (set-ebp val x86)) (logext 64 val)) :hints (("Goal" :in-theory (enable ebp set-ebp))))
+(defthm eax-of-set-eax (equal (eax (set-eax val x86)) (bvchop 32 val)) :hints (("Goal" :in-theory (enable eax set-eax))))
+(defthm ebx-of-set-ebx (equal (ebx (set-ebx val x86)) (bvchop 32 val)) :hints (("Goal" :in-theory (enable ebx set-ebx))))
+(defthm ecx-of-set-ecx (equal (ecx (set-ecx val x86)) (bvchop 32 val)) :hints (("Goal" :in-theory (enable ecx set-ecx))))
+(defthm edx-of-set-edx (equal (edx (set-edx val x86)) (bvchop 32 val)) :hints (("Goal" :in-theory (enable edx set-edx))))
+(defthm esp-of-set-esp (equal (esp (set-esp val x86)) (bvchop 32 val)) :hints (("Goal" :in-theory (enable esp set-esp))))
+(defthm ebp-of-set-ebp (equal (ebp (set-ebp val x86)) (bvchop 32 val)) :hints (("Goal" :in-theory (enable ebp set-ebp))))
 
 ;; Read of a write of a different register
 
@@ -130,7 +253,13 @@
 (defthm ebp-of-set-edx (equal (ebp (set-edx val x86)) (ebp x86)) :hints (("Goal" :in-theory (enable ebp set-edx))))
 (defthm ebp-of-set-esp (equal (ebp (set-esp val x86)) (ebp x86)) :hints (("Goal" :in-theory (enable ebp set-esp))))
 
-;;;
+;;; readers ignore set-reg-high
+(defthm eax-of-set-reg-high (equal (eax (set-reg-high reg val x86)) (eax x86)) :hints (("Goal" :in-theory (enable eax set-reg-high))))
+(defthm ebx-of-set-reg-high (equal (ebx (set-reg-high reg val x86)) (ebx x86)) :hints (("Goal" :in-theory (enable ebx set-reg-high))))
+(defthm ecx-of-set-reg-high (equal (ecx (set-reg-high reg val x86)) (ecx x86)) :hints (("Goal" :in-theory (enable ecx set-reg-high))))
+(defthm edx-of-set-reg-high (equal (edx (set-reg-high reg val x86)) (edx x86)) :hints (("Goal" :in-theory (enable edx set-reg-high))))
+(defthm esp-of-set-reg-high (equal (esp (set-reg-high reg val x86)) (esp x86)) :hints (("Goal" :in-theory (enable esp set-reg-high))))
+(defthm ebp-of-set-reg-high (equal (ebp (set-reg-high reg val x86)) (ebp x86)) :hints (("Goal" :in-theory (enable ebp set-reg-high))))
 
 (defthm xr-of-set-eax
   (implies (or (not (equal fld :rgf))
@@ -185,6 +314,13 @@
            (equal (xr fld index (set-eip eip x86))
                   (xr fld index x86))))
 
+;; needed when fld is :seg-hidden-limit
+(defthm xr-of-set-reg-high-irrel
+  (implies (not (equal fld :rgf))
+           (equal (xr fld index (set-reg-high reg val x86))
+                  (xr fld index x86)))
+  :hints (("Goal" :in-theory (enable set-reg-high))))
+
 ;drop?
 (defthm xr-of-set-eip-same
   (equal (xr :rip nil (set-eip eip x86))
@@ -199,7 +335,7 @@
                )
            (equal (set-eax eax (xw fld index val x86))
                   (xw fld index val (set-eax eax x86))))
-  :hints (("Goal" :in-theory (enable set-eax
+  :hints (("Goal" :in-theory (enable set-eax rax-high
                                      ))))
 
 (defthm set-ebx-of-xw
@@ -208,7 +344,7 @@
                )
            (equal (set-ebx ebx (xw fld index val x86))
                   (xw fld index val (set-ebx ebx x86))))
-  :hints (("Goal" :in-theory (enable set-ebx
+  :hints (("Goal" :in-theory (enable set-ebx rbx-high
                                      ))))
 
 (defthm set-ecx-of-xw
@@ -217,7 +353,7 @@
                )
            (equal (set-ecx ecx (xw fld index val x86))
                   (xw fld index val (set-ecx ecx x86))))
-  :hints (("Goal" :in-theory (enable set-ecx
+  :hints (("Goal" :in-theory (enable set-ecx rcx-high
                                      ))))
 
 (defthm set-edx-of-xw
@@ -226,7 +362,7 @@
                )
            (equal (set-edx edx (xw fld index val x86))
                   (xw fld index val (set-edx edx x86))))
-  :hints (("Goal" :in-theory (enable set-edx
+  :hints (("Goal" :in-theory (enable set-edx rdx-high
                                      ))))
 
 (defthm set-esp-of-xw
@@ -235,7 +371,7 @@
                )
            (equal (set-esp esp (xw fld index val x86))
                   (xw fld index val (set-esp esp x86))))
-  :hints (("Goal" :in-theory (enable set-esp
+  :hints (("Goal" :in-theory (enable set-esp rsp-high
                                      ))))
 
 (defthm set-ebp-of-xw
@@ -244,7 +380,7 @@
                )
            (equal (set-ebp ebp (xw fld index val x86))
                   (xw fld index val (set-ebp ebp x86))))
-  :hints (("Goal" :in-theory (enable set-ebp
+  :hints (("Goal" :in-theory (enable set-ebp rbp-high
                                      ))))
 
 ;;;
@@ -256,172 +392,125 @@
 (defthm set-ebx-of-set-eax
   (equal (set-ebx ebx (set-eax eax x86))
          (set-eax eax (set-ebx ebx x86)))
-  :hints (("Goal" :in-theory (enable set-eax set-ebx
-                                     ))))
+  :hints (("Goal" :in-theory (enable set-eax set-ebx rax-high rbx-high))))
 
 (defthm set-ecx-of-set-eax
   (equal (set-ecx ecx (set-eax eax x86))
          (set-eax eax (set-ecx ecx x86)))
-  :hints (("Goal" :in-theory (enable set-eax set-ecx
-                                     ))))
+  :hints (("Goal" :in-theory (enable set-eax set-ecx rax-high rcx-high))))
 
 (defthm set-edx-of-set-eax
   (equal (set-edx edx (set-eax eax x86))
          (set-eax eax (set-edx edx x86)))
-  :hints (("Goal" :in-theory (enable set-eax set-edx
-                                     ))))
+  :hints (("Goal" :in-theory (enable set-eax set-edx rax-high rdx-high))))
 
 (defthm set-esp-of-set-eax
   (equal (set-esp esp (set-eax eax x86))
          (set-eax eax (set-esp esp x86)))
-  :hints (("Goal" :in-theory (enable set-eax set-esp
-                                     ))))
+  :hints (("Goal" :in-theory (enable set-eax set-esp rax-high rsp-high))))
 
 (defthm set-ebp-of-set-eax
   (equal (set-ebp ebp (set-eax eax x86))
          (set-eax eax (set-ebp ebp x86)))
-  :hints (("Goal" :in-theory (enable set-eax set-ebp
-                                     ))))
+  :hints (("Goal" :in-theory (enable set-eax set-ebp rax-high rbp-high))))
 
 ;;; bring set-ebx forward
 
 (defthm set-ecx-of-set-ebx
   (equal (set-ecx ecx (set-ebx ebx x86))
          (set-ebx ebx (set-ecx ecx x86)))
-  :hints (("Goal" :in-theory (enable set-ebx set-ecx
-                                     ))))
+  :hints (("Goal" :in-theory (enable set-ebx set-ecx rbx-high rcx-high))))
 
 (defthm set-edx-of-set-ebx
   (equal (set-edx edx (set-ebx ebx x86))
          (set-ebx ebx (set-edx edx x86)))
-  :hints (("Goal" :in-theory (enable set-ebx set-edx
-                                     ))))
+  :hints (("Goal" :in-theory (enable set-ebx set-edx rbx-high rdx-high))))
 
 (defthm set-esp-of-set-ebx
   (equal (set-esp esp (set-ebx ebx x86))
          (set-ebx ebx (set-esp esp x86)))
-  :hints (("Goal" :in-theory (enable set-ebx set-esp
-                                     ))))
+  :hints (("Goal" :in-theory (enable set-ebx set-esp rbx-high rsp-high))))
 
 (defthm set-ebp-of-set-ebx
   (equal (set-ebp ebp (set-ebx ebx x86))
          (set-ebx ebx (set-ebp ebp x86)))
-  :hints (("Goal" :in-theory (enable set-ebx set-ebp
-                                     ))))
+  :hints (("Goal" :in-theory (enable set-ebx set-ebp rbx-high rbp-high))))
 
 ;;; bring set-ecx forward
 
 (defthm set-edx-of-set-ecx
   (equal (set-edx edx (set-ecx ecx x86))
          (set-ecx ecx (set-edx edx x86)))
-  :hints (("Goal" :in-theory (enable set-ecx set-edx
-                                     ))))
+  :hints (("Goal" :in-theory (enable set-ecx set-edx rcx-high rdx-high))))
 
 (defthm set-esp-of-set-ecx
   (equal (set-esp esp (set-ecx ecx x86))
          (set-ecx ecx (set-esp esp x86)))
-  :hints (("Goal" :in-theory (enable set-ecx set-esp
-                                     ))))
+  :hints (("Goal" :in-theory (enable set-ecx set-esp rcx-high rsp-high))))
 
 (defthm set-ebp-of-set-ecx
   (equal (set-ebp ebp (set-ecx ecx x86))
          (set-ecx ecx (set-ebp ebp x86)))
-  :hints (("Goal" :in-theory (enable set-ecx set-ebp
-                                     ))))
+  :hints (("Goal" :in-theory (enable set-ecx set-ebp rcx-high rbp-high))))
 
 ;;; bring set-edx forward
 
 (defthm set-esp-of-set-edx
   (equal (set-esp esp (set-edx edx x86))
          (set-edx edx (set-esp esp x86)))
-  :hints (("Goal" :in-theory (enable set-edx set-esp
-                                     ))))
+  :hints (("Goal" :in-theory (enable set-edx set-esp rdx-high rsp-high))))
 
 (defthm set-ebp-of-set-edx
   (equal (set-ebp ebp (set-edx edx x86))
          (set-edx edx (set-ebp ebp x86)))
-  :hints (("Goal" :in-theory (enable set-edx set-ebp
-                                     ))))
+  :hints (("Goal" :in-theory (enable set-edx set-ebp rdx-high rbp-high))))
 
 ;;; bring set-esp forward
 
 (defthm set-ebp-of-set-esp
   (equal (set-ebp ebp (set-esp esp x86))
          (set-esp esp (set-ebp ebp x86)))
-  :hints (("Goal" :in-theory (enable set-esp set-ebp
-                                     ))))
+  :hints (("Goal" :in-theory (enable set-esp set-ebp rsp-high rbp-high))))
 
 ;; Write of write of the same register
-(defthm set-eax-of-set-eax (equal (set-eax eax1 (set-eax eax2 x86)) (set-eax eax1 x86)) :hints (("Goal" :in-theory (enable set-eax))))
-(defthm set-ebx-of-set-ebx (equal (set-ebx ebx1 (set-ebx ebx2 x86)) (set-ebx ebx1 x86)) :hints (("Goal" :in-theory (enable set-ebx))))
-(defthm set-ecx-of-set-ecx (equal (set-ecx ecx1 (set-ecx ecx2 x86)) (set-ecx ecx1 x86)) :hints (("Goal" :in-theory (enable set-ecx))))
-(defthm set-edx-of-set-edx (equal (set-edx edx1 (set-edx edx2 x86)) (set-edx edx1 x86)) :hints (("Goal" :in-theory (enable set-edx))))
-(defthm set-esp-of-set-esp (equal (set-esp esp1 (set-esp esp2 x86)) (set-esp esp1 x86)) :hints (("Goal" :in-theory (enable set-esp))))
-(defthm set-ebp-of-set-ebp (equal (set-ebp ebp1 (set-ebp ebp2 x86)) (set-ebp ebp1 x86)) :hints (("Goal" :in-theory (enable set-ebp))))
-
-;; Introduce the register readers:
-;; These rules are disabled since they are not appropriate for 64-bit reasoning:
-(defthmd xr-becomes-eax (equal (xr :rgf *rax* x86) (eax x86)) :hints (("Goal" :in-theory (enable eax))))
-(defthmd xr-becomes-ebx (equal (xr :rgf *rbx* x86) (ebx x86)) :hints (("Goal" :in-theory (enable ebx))))
-(defthmd xr-becomes-ecx (equal (xr :rgf *rcx* x86) (ecx x86)) :hints (("Goal" :in-theory (enable ecx))))
-(defthmd xr-becomes-edx (equal (xr :rgf *rdx* x86) (edx x86)) :hints (("Goal" :in-theory (enable edx))))
-(defthmd xr-becomes-esp (equal (xr :rgf *rsp* x86) (esp x86)) :hints (("Goal" :in-theory (enable esp))))
-(defthmd xr-becomes-ebp (equal (xr :rgf *rbp* x86) (ebp x86)) :hints (("Goal" :in-theory (enable ebp))))
-
-(theory-invariant (incompatible (:definition eax) (:rewrite xr-becomes-eax)))
-(theory-invariant (incompatible (:definition ebx) (:rewrite xr-becomes-ebx)))
-(theory-invariant (incompatible (:definition ecx) (:rewrite xr-becomes-ecx)))
-(theory-invariant (incompatible (:definition edx) (:rewrite xr-becomes-edx)))
-(theory-invariant (incompatible (:definition esp) (:rewrite xr-becomes-esp)))
-(theory-invariant (incompatible (:definition ebp) (:rewrite xr-becomes-ebp)))
-
-;; Introduce the register writers:
-;; These rules are disabled since they are not appropriate for 64-bit reasoning:
-(defthmd xw-becomes-set-eax (equal (xw :rgf *rax* val x86) (set-eax val x86)) :hints (("Goal" :in-theory (enable set-eax))))
-(defthmd xw-becomes-set-ebx (equal (xw :rgf *rbx* val x86) (set-ebx val x86)) :hints (("Goal" :in-theory (enable set-ebx))))
-(defthmd xw-becomes-set-ecx (equal (xw :rgf *rcx* val x86) (set-ecx val x86)) :hints (("Goal" :in-theory (enable set-ecx))))
-(defthmd xw-becomes-set-edx (equal (xw :rgf *rdx* val x86) (set-edx val x86)) :hints (("Goal" :in-theory (enable set-edx))))
-(defthmd xw-becomes-set-esp (equal (xw :rgf *rsp* val x86) (set-esp val x86)) :hints (("Goal" :in-theory (enable set-esp))))
-(defthmd xw-becomes-set-ebp (equal (xw :rgf *rbp* val x86) (set-ebp val x86)) :hints (("Goal" :in-theory (enable set-ebp))))
-
-(theory-invariant (incompatible (:definition set-eax) (:rewrite xw-becomes-set-eax)))
-(theory-invariant (incompatible (:definition set-ebx) (:rewrite xw-becomes-set-ebx)))
-(theory-invariant (incompatible (:definition set-ecx) (:rewrite xw-becomes-set-ecx)))
-(theory-invariant (incompatible (:definition set-edx) (:rewrite xw-becomes-set-edx)))
-(theory-invariant (incompatible (:definition set-esp) (:rewrite xw-becomes-set-esp)))
-(theory-invariant (incompatible (:definition set-ebp) (:rewrite xw-becomes-set-ebp)))
+(defthm set-eax-of-set-eax (equal (set-eax eax1 (set-eax eax2 x86)) (set-eax eax1 x86)) :hints (("Goal" :in-theory (enable set-eax rax-high))))
+(defthm set-ebx-of-set-ebx (equal (set-ebx ebx1 (set-ebx ebx2 x86)) (set-ebx ebx1 x86)) :hints (("Goal" :in-theory (enable set-ebx rbx-high))))
+(defthm set-ecx-of-set-ecx (equal (set-ecx ecx1 (set-ecx ecx2 x86)) (set-ecx ecx1 x86)) :hints (("Goal" :in-theory (enable set-ecx rcx-high))))
+(defthm set-edx-of-set-edx (equal (set-edx edx1 (set-edx edx2 x86)) (set-edx edx1 x86)) :hints (("Goal" :in-theory (enable set-edx rdx-high))))
+(defthm set-esp-of-set-esp (equal (set-esp esp1 (set-esp esp2 x86)) (set-esp esp1 x86)) :hints (("Goal" :in-theory (enable set-esp rsp-high))))
+(defthm set-ebp-of-set-ebp (equal (set-ebp ebp1 (set-ebp ebp2 x86)) (set-ebp ebp1 x86)) :hints (("Goal" :in-theory (enable set-ebp rbp-high))))
 
 ;;; todo: can we get rid of these?
 
-(defthm xr-of-set-esp-same
-  (equal (xr ':rgf '4 (set-esp esp x86))
-         (logext 64 esp))
-  :hints (("Goal" :in-theory (enable set-esp))))
+;; (defthm xr-of-set-esp-same
+;;   (equal (xr ':rgf '4 (set-esp esp x86))
+;;          (bvchop 32 esp))
+;;   :hints (("Goal" :in-theory (enable set-esp rsp-high))))
 
-(defthm xr-of-esp-and-set-eax
-  (equal (xr ':rgf '4 (set-eax esp x86))
-         (xr ':rgf '4 x86))
-  :hints (("Goal" :in-theory (enable set-eax))))
+;; (defthm xr-of-esp-and-set-eax
+;;   (equal (xr ':rgf '4 (set-eax esp x86))
+;;          (xr ':rgf '4 x86))
+;;   :hints (("Goal" :in-theory (enable set-eax))))
 
-(defthm xr-of-esp-and-set-ebx
-  (equal (xr ':rgf '4 (set-ebx esp x86))
-         (xr ':rgf '4 x86))
-  :hints (("Goal" :in-theory (enable set-ebx))))
+;; (defthm xr-of-esp-and-set-ebx
+;;   (equal (xr ':rgf '4 (set-ebx esp x86))
+;;          (xr ':rgf '4 x86))
+;;   :hints (("Goal" :in-theory (enable set-ebx))))
 
-(defthm xr-of-esp-and-set-ecx
-  (equal (xr ':rgf '4 (set-ecx esp x86))
-         (xr ':rgf '4 x86))
-  :hints (("Goal" :in-theory (enable set-ecx))))
+;; (defthm xr-of-esp-and-set-ecx
+;;   (equal (xr ':rgf '4 (set-ecx esp x86))
+;;          (xr ':rgf '4 x86))
+;;   :hints (("Goal" :in-theory (enable set-ecx))))
 
-(defthm xr-of-esp-and-set-edx
-  (equal (xr ':rgf '4 (set-edx esp x86))
-         (xr ':rgf '4 x86))
-  :hints (("Goal" :in-theory (enable set-edx))))
+;; (defthm xr-of-esp-and-set-edx
+;;   (equal (xr ':rgf '4 (set-edx esp x86))
+;;          (xr ':rgf '4 x86))
+;;   :hints (("Goal" :in-theory (enable set-edx))))
 
-(defthm xr-of-esp-and-set-ebp
-  (equal (xr ':rgf '4 (set-ebp ebp x86))
-         (xr ':rgf '4 x86))
-  :hints (("Goal" :in-theory (enable set-ebp))))
+;; (defthm xr-of-esp-and-set-ebp
+;;   (equal (xr ':rgf '4 (set-ebp ebp x86))
+;;          (xr ':rgf '4 x86))
+;;   :hints (("Goal" :in-theory (enable set-ebp))))
 
 ;;;
 
